feat(library/init/algebra/classes): add is_strict_total_order type class

library/init/algebra/classes.lean
@@ -112,6 +112,8 @@ instance is_total_preorder_is_preorder (α : Type u) (r : α → α → Prop) [s
 @[algebra] class is_trichotomous (α : Type u) (lt : α → α → Prop) : Prop :=
 (trichotomous : ∀ a b, lt a b ∨ a = b ∨ lt b a)
 
+@[algebra] class is_strict_total_order (α : Type u) (lt : α → α → Prop) extends is_trichotomous α lt, is_strict_weak_order α lt.
+
 instance eq_is_equiv (α : Type u) : is_equiv α (=) :=
 {symm := @eq.symm _, trans := @eq.trans _, refl := eq.refl}
 
